runtime/test/tree_test.ml
@@ -44,9 +44,39 @@ let bench_main () =
   print_string "\nBenchmarks...\n";
   compare_time_loop (fun n -> make false n 2)
                     40 1 2
-                    (fun t -> Marshal.to_bytes t [])
-                    (fun w -> Atom false)
-       
-let _ = test_main ();
-        space_main ();
-        bench_main ()
+                    tree_serialize_top
+                    (fun w -> match tree_deserialize_top w with
+                              | Some p -> p
+                              | None -> failwith "Deserialization failed")
+                    
+                    
+let avg_time_height (f : 'a tree -> 'b) (h : int) =
+  let num_tries = 100 in
+  avg (time_loop (fun n -> make false n 2) h num_tries f)
+
+let compare_map_main () =
+  let max_height = 25 in
+  let rec loop i =
+    if i < max_height
+    then let map_avg = avg_time_height (map0 (fun _ -> ())) i in
+         let tr_map_avg = avg_time_height (tree_map' (fun _ -> ())) i in
+         (Printf.printf "map: %f, tail-rec map: %f \n" map_avg tr_map_avg;
+          loop (i + 1)) in
+  loop 0
+
+let compare_serialize_tr_main () =
+  let max_height = 25 in
+  let rec loop i =
+    if i < max_height
+    then let s_avg = avg_time_height (fun t -> t) i in
+         let tr_s_avg = avg_time_height tree_serialize_top' i in
+         (Printf.printf "height: %d, serialize: %f, tail-rec serialize: %f \n"
+                        i s_avg tr_s_avg;
+          loop (i + 1)) in
+  loop 0
+                    
+let main () = test_main ();
+              space_main ();
+              bench_main ()
+
+let _ = compare_serialize_tr_main ()
