runtime/coq/ExtractTreeSerializer.v
@@ -1,4 +1,5 @@
 Require Import Cheerios.ExtractTreeSerializerDeps.
+Require Import Cheerios.BasicSerializers.
 
 Require Import ZArith.
 Require Import ExtrOcamlBasic.
@@ -10,5 +11,10 @@ Definition tree_serialize_top : tree bool -> Serializer.wire :=
 Definition tree_deserialize_top : Serializer.wire -> option (tree bool) :=
   deserialize_top deserialize.
 
+Definition tree_serialize_top' (t : tree bool) : Serializer.wire :=
+  Serializer.wire_wrap (tree_serialize' _ t).
+
 Extraction "runtime/ocaml/tree_serializer.ml"
+           map tree_map'
+           tree_serialize_top'
            tree_serialize_top tree_deserialize_top.
